examples/cms/common.v
@@ -1,0 +1,156 @@
+Require Import Poulet4.P4light.Syntax.P4defs.
+Require Import Poulet4.P4light.Semantics.Semantics.
+Require Import Coq.Program.Program.
+Require Import ProD3.core.Core.
+Require Import ProD3.core.Tofino.
+Require Import ProD3.examples.cms.p4ast.
+Require Import ProD3.examples.cms.ConModel.
+
+Open Scope func_spec.
+
+Notation ident := string.
+Notation path := (list ident).
+Notation Val := (@ValueBase bool).
+Notation Sval := (@ValueBase (option bool)).
+
+Definition am_ge := ltac:(get_am_ge prog).
+Definition ge := ltac:(get_ge am_ge prog).
+
+(* Constants *)
+
+Definition NOOP := 0.
+Definition CLEAR := 1.
+Definition INSERT := 2.
+Definition QUERY := 3.
+Definition INSQUERY := 4.
+
+Definition index_w := 15%N.
+Definition value_w := 32%N.
+Definition num_slots := Eval compute in 2 ^ (Z.of_N index_w).
+Definition num_rows := 4.
+Definition num_frames := 4.
+Definition frame_tick_tocks := 56.
+Definition tick_time := 268435456.
+Definition frame_time := frame_tick_tocks * tick_time * 2.
+
+Definition poly1 : Tofino.CRC_polynomial :=
+  {|
+    Tofino.CRCP_width := 32;
+    Tofino.CRCP_coeff := P4Arith.to_lbool 32 79764919;
+    Tofino.CRCP_reversed := true;
+    Tofino.CRCP_msb := false;
+    Tofino.CRCP_extended := false;
+    Tofino.CRCP_init := P4Arith.to_lbool 32 0;
+    Tofino.CRCP_xor := P4Arith.to_lbool 32 4294967295
+  |}.
+
+Definition hash1 (v : Val) :=
+  hash_Z 32 poly1 v mod 2 ^ (Z.of_N index_w).
+
+Definition poly2 : Tofino.CRC_polynomial :=
+  {|
+    Tofino.CRCP_width := 32;
+    Tofino.CRCP_coeff := P4Arith.to_lbool 32 517762881;
+    Tofino.CRCP_reversed := true;
+    Tofino.CRCP_msb := false;
+    Tofino.CRCP_extended := false;
+    Tofino.CRCP_init := P4Arith.to_lbool 32 0;
+    Tofino.CRCP_xor := P4Arith.to_lbool 32 4294967295
+  |}.
+
+Definition hash2 (v : Val) :=
+  hash_Z 32 poly2 v mod 2 ^ Z.of_N index_w.
+
+
+Definition poly3 : Tofino.CRC_polynomial :=
+  {|
+    Tofino.CRCP_width := 32;
+    Tofino.CRCP_coeff := P4Arith.to_lbool 32 2821953579;
+    Tofino.CRCP_reversed := true;
+    Tofino.CRCP_msb := false;
+    Tofino.CRCP_extended := false;
+    Tofino.CRCP_init := P4Arith.to_lbool 32 0;
+    Tofino.CRCP_xor := P4Arith.to_lbool 32 4294967295
+  |}.
+
+Definition hash3 (v : Val) :=
+  hash_Z 32 poly3 v mod 2 ^ Z.of_N index_w.
+
+(* Placeholder *)
+Definition hash4 := hash3.
+
+Definition header_type : Set := Z * Z.
+
+Definition header_to_val '((x, y) : header_type) : Val :=
+  ValBaseBit ((P4Arith.to_lbool 32 y) ++ (P4Arith.to_lbool 32 x)).
+
+Definition hashes := [hash1 ∘ header_to_val; hash2 ∘ header_to_val; hash3 ∘ header_to_val; hash4 ∘ header_to_val].
+
+Lemma H_Zlength_hashes : Zlength hashes = num_rows.
+Proof. auto. Qed.
+
+Lemma b2z_range : forall b,
+  0 <= Z.b2z b < 2.
+Proof.
+  destruct b; simpl; lia.
+Qed.
+
+Ltac add_b2z_range b :=
+  assert_fails (assert (0 <= Z.b2z b < 2) by assumption);
+  pose proof (b2z_range b).
+
+Ltac saturate_b2z :=
+  repeat match goal with
+  | H : context [Z.b2z ?b] |- _ =>
+      add_b2z_range b
+  | |- context [Z.b2z ?b] =>
+      add_b2z_range b
+  end.
+
+Ltac Zify.zify_pre_hook ::=
+  unfold is_true, index_w, num_slots, num_rows, num_frames, frame_tick_tocks,
+    NOOP, CLEAR, INSERT, QUERY, INSQUERY in *;
+  saturate_b2z.
+
+Definition rows := ["row_1"; "row_2"; "row_3"; "row_4"].
+Definition panes := ["win_1"; "win_2"; "win_3"; "win_4"].
+
+Definition H_num_slots : 0 < num_slots := eq_refl.
+Definition H_num_rows : 0 < num_rows := eq_refl.
+Definition H_num_frames : 1 < num_frames := eq_refl.
+
+Notation row := (row num_slots).
+Notation frame := (frame num_rows num_slots).
+
+#[export] Instance Inhabitant_row : Inhabitant row :=
+  Inhabitant_row H_num_slots.
+
+#[export] Instance Inhabitant_frame : Inhabitant frame :=
+  Inhabitant_frame H_num_rows H_num_slots.
+
+(* NoAction *)
+
+Definition NoAction_fundef : @fundef Info :=
+  ltac:(get_fd ["NoAction"] ge).
+
+Definition NoAction_spec : func_spec :=
+  WITH,
+    PATH []
+    MOD None []
+    WITH,
+      PRE
+        (ARG []
+        (MEM []
+        (EXT [])))
+      POST
+        (ARG_RET [] ValBaseNull
+        (MEM []
+        (EXT []))).
+
+Lemma NoAction_body :
+  func_sound ge NoAction_fundef nil NoAction_spec.
+Proof.
+  start_function.
+  step.
+  entailer.
+Qed.
