examples/cms/verif_Win1.v
@@ -1,0 +1,870 @@
+Require Import Poulet4.P4light.Syntax.P4defs.
+Require Import Poulet4.P4light.Semantics.Semantics.
+Require Import ProD3.core.Core.
+Require Import ProD3.core.Tofino.
+Require Import ProD3.examples.cms.ConModel.
+Require Import ProD3.examples.cms.common.
+Require Import ProD3.examples.cms.ModelRepr.
+Require Import ProD3.examples.cms.verif_Row11.
+Require Import ProD3.examples.cms.verif_Row12.
+Require Import ProD3.examples.cms.verif_Row13.
+Require Import ProD3.examples.cms.verif_Row14.
+Require Import Hammer.Plugin.Hammer.
+Require Export Coq.Program.Program.
+Import ListNotations.
+
+Notation ident := string.
+Notation path := (list ident).
+Notation Val := (@ValueBase bool).
+Notation Sval := (@ValueBase (option bool)).
+
+Definition p := ["pipe"; "ingress"; "cm2_ds"; "win_1"].
+
+Definition P4min a b := Z.min (P4Arith.BitArith.mod_bound value_w a) (P4Arith.BitArith.mod_bound value_w b).
+
+Definition min_spec : func_spec :=
+  WITH,
+    PATH []
+    MOD None []
+    WITH (a b : Z),
+      PRE
+        (ARG [P4Bit value_w a; P4Bit value_w b]
+        (MEM []
+        (EXT [])))
+      POST
+        (ARG_RET [] (P4Bit value_w (P4min a b))
+        (MEM []
+        (EXT []))).
+
+Lemma min_body :
+  func_sound ge (FExternal "" "min") [TypBit value_w] min_spec.
+Admitted.
+
+#[local] Hint Extern 5 (func_modifies _ _ _ _ _) => (apply min_body) : func_specs.
+
+Definition act_merge_rows_1_fd :=
+  ltac:(get_fd ["Cm2CountMinSketchWin"; "act_merge_rows_1"] ge).
+
+Definition act_merge_rows_1_spec : func_spec :=
+  WITH (* p *),
+    PATH p
+    MOD (Some [["win_md"]]) []
+    WITH api_call index_1 index_2 index_3 index_4 rw_1 rw_2 rw_3 rw_4,
+      PRE
+        (ARG []
+        (MEM [(["win_md"], ValBaseStruct
+               [("api_call", api_call);
+                ("index_1", index_1);
+                ("index_2", index_2);
+                ("index_3", index_3);
+                ("index_4", index_4);
+                ("rw_1", P4Bit value_w rw_1);
+                ("rw_2", P4Bit value_w rw_2);
+                ("rw_3", P4Bit value_w rw_3);
+                ("rw_4", P4Bit value_w rw_4)
+               ])
+             ]
+        (EXT [])))
+      POST
+        (ARG_RET [] ValBaseNull
+        (MEM [(["win_md"], ValBaseStruct
+               [("api_call", api_call);
+                ("index_1", index_1);
+                ("index_2", index_2);
+                ("index_3", index_3);
+                ("index_4", index_4);
+                ("rw_1", P4Bit value_w (P4min rw_1 rw_3));
+                ("rw_2", P4Bit value_w (P4min rw_2 rw_4));
+                ("rw_3", P4Bit value_w rw_3);
+                ("rw_4", P4Bit value_w rw_4)
+               ])
+             ]
+        (EXT []))).
+
+Lemma act_merge_rows_1_body :
+  func_sound ge act_merge_rows_1_fd nil act_merge_rows_1_spec.
+Proof.
+  start_function.
+  step_call min_body.
+  { entailer. }
+  step_call min_body.
+  { entailer. }
+  step.
+  entailer.
+Qed.
+
+#[local] Hint Extern 5 (func_modifies _ _ _ _ _) => (apply act_merge_rows_1_body) : func_specs.
+
+Definition act_merge_rows_2_fd :=
+  ltac:(get_fd ["Cm2CountMinSketchWin"; "act_merge_rows_2"] ge).
+
+Definition act_merge_rows_2_spec : func_spec :=
+  WITH (* p *),
+    PATH p
+    MOD (Some [["win_md"]]) []
+    WITH api_call index_1 index_2 index_3 index_4 rw_1 rw_2 rw_3 rw_4,
+      PRE
+        (ARG []
+        (MEM [(["win_md"], ValBaseStruct
+               [("api_call", api_call);
+                ("index_1", index_1);
+                ("index_2", index_2);
+                ("index_3", index_3);
+                ("index_4", index_4);
+                ("rw_1", P4Bit value_w rw_1);
+                ("rw_2", P4Bit value_w rw_2);
+                ("rw_3", rw_3);
+                ("rw_4", rw_4)
+               ])
+             ]
+        (EXT [])))
+      POST
+        (ARG_RET [] ValBaseNull
+        (MEM [(["win_md"], ValBaseStruct
+               [("api_call", api_call);
+                ("index_1", index_1);
+                ("index_2", index_2);
+                ("index_3", index_3);
+                ("index_4", index_4);
+                ("rw_1", P4Bit value_w (P4min rw_1 rw_2));
+                ("rw_2", P4Bit value_w rw_2);
+                ("rw_3", rw_3);
+                ("rw_4", rw_4)
+               ])
+             ]
+        (EXT []))).
+
+Lemma act_merge_rows_2_body :
+  func_sound ge act_merge_rows_2_fd nil act_merge_rows_2_spec.
+Proof.
+  start_function.
+  step_call min_body.
+  { entailer. }
+  step.
+  entailer.
+Qed.
+
+#[local] Hint Extern 5 (func_modifies _ _ _ _ _) => (apply act_merge_rows_2_body) : func_specs.
+
+Definition tbl_merge_rows_1_fd :=
+  ltac:(get_fd ["Cm2CountMinSketchWin"; "tbl_merge_rows_1"; "apply"] ge).
+
+Definition tbl_merge_rows_1_spec : func_spec :=
+  WITH (* p *),
+    PATH p
+    MOD (Some [["win_md"]]) []
+    WITH api_call index_1 index_2 index_3 index_4 rw_1 rw_2 rw_3 rw_4,
+      PRE
+        (ARG []
+        (MEM [(["win_md"], ValBaseStruct
+               [("api_call", api_call);
+                ("index_1", index_1);
+                ("index_2", index_2);
+                ("index_3", index_3);
+                ("index_4", index_4);
+                ("rw_1", P4Bit value_w rw_1);
+                ("rw_2", P4Bit value_w rw_2);
+                ("rw_3", P4Bit value_w rw_3);
+                ("rw_4", P4Bit value_w rw_4)
+               ])
+             ]
+        (EXT [])))
+      POST
+        (EX retv,
+        (ARG_RET [] retv
+        (MEM [(["win_md"], ValBaseStruct
+               [("api_call", api_call);
+                ("index_1", index_1);
+                ("index_2", index_2);
+                ("index_3", index_3);
+                ("index_4", index_4);
+                ("rw_1", P4Bit value_w (P4min rw_1 rw_3));
+                ("rw_2", P4Bit value_w (P4min rw_2 rw_4));
+                ("rw_3", P4Bit value_w rw_3);
+                ("rw_4", P4Bit value_w rw_4)
+               ])
+             ]
+        (EXT []))))%arg_ret_assr.
+
+Lemma tbl_merge_rows_1_body :
+  func_sound ge tbl_merge_rows_1_fd nil tbl_merge_rows_1_spec.
+Proof.
+  start_function.
+  table_action act_merge_rows_1_body.
+  { entailer. }
+  { entailer. }
+Qed.
+
+#[local] Hint Extern 5 (func_modifies _ _ _ _ _) => (apply tbl_merge_rows_1_body) : func_specs.
+
+Definition tbl_merge_rows_2_fd :=
+  ltac:(get_fd ["Cm2CountMinSketchWin"; "tbl_merge_rows_2"; "apply"] ge).
+
+Definition tbl_merge_rows_2_spec : func_spec :=
+  WITH (* p *),
+    PATH p
+    MOD (Some [["win_md"]]) []
+    WITH api_call index_1 index_2 index_3 index_4 rw_1 rw_2 rw_3 rw_4,
+      PRE
+        (ARG []
+        (MEM [(["win_md"], ValBaseStruct
+               [("api_call", api_call);
+                ("index_1", index_1);
+                ("index_2", index_2);
+                ("index_3", index_3);
+                ("index_4", index_4);
+                ("rw_1", P4Bit value_w rw_1);
+                ("rw_2", P4Bit value_w rw_2);
+                ("rw_3", rw_3);
+                ("rw_4", rw_4)
+               ])
+             ]
+        (EXT [])))
+      POST
+        (EX retv,
+        (ARG_RET [] retv
+        (MEM [(["win_md"], ValBaseStruct
+               [("api_call", api_call);
+                ("index_1", index_1);
+                ("index_2", index_2);
+                ("index_3", index_3);
+                ("index_4", index_4);
+                ("rw_1", P4Bit value_w (P4min rw_1 rw_2));
+                ("rw_2", P4Bit value_w rw_2);
+                ("rw_3", rw_3);
+                ("rw_4", rw_4)
+               ])
+             ]
+        (EXT []))))%arg_ret_assr.
+
+Lemma tbl_merge_rows_2_body :
+  func_sound ge tbl_merge_rows_2_fd nil tbl_merge_rows_2_spec.
+Proof.
+  start_function.
+  table_action act_merge_rows_2_body.
+  { entailer. }
+  { entailer. }
+Qed.
+
+#[local] Hint Extern 5 (func_modifies _ _ _ _ _) => (apply tbl_merge_rows_2_body) : func_specs.
+
+Definition min_undef_spec : func_spec :=
+  WITH,
+    PATH []
+    MOD None []
+    WITH,
+      PRE
+        (ARG [P4Bit_ value_w; P4Bit_ value_w]
+        (MEM []
+        (EXT [])))
+      POST
+        (ARG_RET [] (P4Bit_ value_w)
+        (MEM []
+        (EXT []))).
+
+Lemma min_undef_body :
+  func_sound ge (FExternal "" "min") [TypBit value_w] min_undef_spec.
+Admitted.
+
+Definition act_merge_rows_1_undef_spec : func_spec :=
+  WITH (* p *),
+    PATH p
+    MOD (Some [["win_md"]]) []
+    WITH api_call index_1 index_2 index_3 index_4,
+      PRE
+        (ARG []
+        (MEM [(["win_md"], ValBaseStruct
+               [("api_call", api_call);
+                ("index_1", index_1);
+                ("index_2", index_2);
+                ("index_3", index_3);
+                ("index_4", index_4);
+                ("rw_1", P4Bit_ value_w);
+                ("rw_2", P4Bit_ value_w);
+                ("rw_3", P4Bit_ value_w);
+                ("rw_4", P4Bit_ value_w)
+               ])
+             ]
+        (EXT [])))
+      POST
+        (ARG_RET [] ValBaseNull
+        (MEM [(["win_md"], ValBaseStruct
+               [("api_call", api_call);
+                ("index_1", index_1);
+                ("index_2", index_2);
+                ("index_3", index_3);
+                ("index_4", index_4);
+                ("rw_1", P4Bit_ value_w);
+                ("rw_2", P4Bit_ value_w);
+                ("rw_3", P4Bit_ value_w);
+                ("rw_4", P4Bit_ value_w)
+               ])
+             ]
+        (EXT []))).
+
+Lemma act_merge_rows_1_undef_body :
+  func_sound ge act_merge_rows_1_fd nil act_merge_rows_1_undef_spec.
+Proof.
+  start_function.
+  step_call min_undef_body.
+  { entailer. }
+  step_call min_undef_body.
+  { entailer. }
+  step.
+  entailer.
+Qed.
+
+Definition act_merge_rows_2_undef_spec : func_spec :=
+  WITH (* p *),
+    PATH p
+    MOD (Some [["win_md"]]) []
+    WITH api_call index_1 index_2 index_3 index_4 rw_3 rw_4,
+      PRE
+        (ARG []
+        (MEM [(["win_md"], ValBaseStruct
+               [("api_call", api_call);
+                ("index_1", index_1);
+                ("index_2", index_2);
+                ("index_3", index_3);
+                ("index_4", index_4);
+                ("rw_1", P4Bit_ value_w);
+                ("rw_2", P4Bit_ value_w);
+                ("rw_3", rw_3);
+                ("rw_4", rw_4)
+               ])
+             ]
+        (EXT [])))
+      POST
+        (ARG_RET [] ValBaseNull
+        (MEM [(["win_md"], ValBaseStruct
+               [("api_call", api_call);
+                ("index_1", index_1);
+                ("index_2", index_2);
+                ("index_3", index_3);
+                ("index_4", index_4);
+                ("rw_1", P4Bit_ value_w);
+                ("rw_2", P4Bit_ value_w);
+                ("rw_3", rw_3);
+                ("rw_4", rw_4)
+               ])
+             ]
+        (EXT []))).
+
+Lemma act_merge_rows_2_undef_body :
+  func_sound ge act_merge_rows_2_fd nil act_merge_rows_2_undef_spec.
+Proof.
+  start_function.
+  step_call min_undef_body.
+  { entailer. }
+  step.
+  entailer.
+Qed.
+
+Definition tbl_merge_rows_1_undef_spec : func_spec :=
+  WITH (* p *),
+    PATH p
+    MOD (Some [["win_md"]]) []
+    WITH api_call index_1 index_2 index_3 index_4,
+      PRE
+        (ARG []
+        (MEM [(["win_md"], ValBaseStruct
+               [("api_call", api_call);
+                ("index_1", index_1);
+                ("index_2", index_2);
+                ("index_3", index_3);
+                ("index_4", index_4);
+                ("rw_1", P4Bit_ value_w);
+                ("rw_2", P4Bit_ value_w);
+                ("rw_3", P4Bit_ value_w);
+                ("rw_4", P4Bit_ value_w)
+               ])
+             ]
+        (EXT [])))
+      POST
+        (EX retv,
+        (ARG_RET [] retv
+        (MEM [(["win_md"], ValBaseStruct
+               [("api_call", api_call);
+                ("index_1", index_1);
+                ("index_2", index_2);
+                ("index_3", index_3);
+                ("index_4", index_4);
+                ("rw_1", P4Bit_ value_w);
+                ("rw_2", P4Bit_ value_w);
+                ("rw_3", P4Bit_ value_w);
+                ("rw_4", P4Bit_ value_w)
+               ])
+             ]
+        (EXT []))))%arg_ret_assr.
+
+Lemma tbl_merge_rows_1_undef_body :
+  func_sound ge tbl_merge_rows_1_fd nil tbl_merge_rows_1_undef_spec.
+Proof.
+  start_function.
+  table_action act_merge_rows_1_undef_body.
+  { entailer. }
+  { entailer. }
+Qed.
+
+Definition tbl_merge_rows_2_undef_spec : func_spec :=
+  WITH (* p *),
+    PATH p
+    MOD (Some [["win_md"]]) []
+    WITH api_call index_1 index_2 index_3 index_4 rw_3 rw_4,
+      PRE
+        (ARG []
+        (MEM [(["win_md"], ValBaseStruct
+               [("api_call", api_call);
+                ("index_1", index_1);
+                ("index_2", index_2);
+                ("index_3", index_3);
+                ("index_4", index_4);
+                ("rw_1", P4Bit_ value_w);
+                ("rw_2", P4Bit_ value_w);
+                ("rw_3", rw_3);
+                ("rw_4", rw_4)
+               ])
+             ]
+        (EXT [])))
+      POST
+        (EX retv,
+        (ARG_RET [] retv
+        (MEM [(["win_md"], ValBaseStruct
+               [("api_call", api_call);
+                ("index_1", index_1);
+                ("index_2", index_2);
+                ("index_3", index_3);
+                ("index_4", index_4);
+                ("rw_1", P4Bit_ value_w);
+                ("rw_2", P4Bit_ value_w);
+                ("rw_3", rw_3);
+                ("rw_4", rw_4)
+               ])
+             ]
+        (EXT []))))%arg_ret_assr.
+
+Lemma tbl_merge_rows_2_undef_body :
+  func_sound ge tbl_merge_rows_2_fd nil tbl_merge_rows_2_undef_spec.
+Proof.
+  start_function.
+  table_action act_merge_rows_2_undef_body.
+  { entailer. }
+  { entailer. }
+Qed.
+
+Definition Win_fundef :=
+  ltac:(get_fd ["Cm2CountMinSketchWin"; "apply"] ge).
+
+Definition Win_noop_spec : func_spec :=
+  WITH (* p *),
+    PATH p
+    MOD None [p]
+    WITH (f : frame) (is : listn Z num_rows)
+      (_ : Forall (fun i => 0 <= i < num_slots) (`is)),
+      PRE
+        (ARG [ValBaseStruct
+               [("api_call", P4Bit 32 NOOP);
+                ("index_1", P4Bit index_w (Znth 0 (`is)));
+                ("index_2", P4Bit index_w (Znth 1 (`is)));
+                ("index_3", P4Bit index_w (Znth 2 (`is)));
+                ("index_4", P4Bit index_w (Znth 3 (`is)));
+                ("rw_1", P4Bit_ value_w);
+                ("rw_2", P4Bit_ value_w);
+                ("rw_3", P4Bit_ value_w);
+                ("rw_4", P4Bit_ value_w)
+               ]
+             ]
+        (MEM []
+        (EXT [frame_repr p rows f])))
+      POST
+        (ARG_RET [ValBaseStruct
+               [("api_call", P4Bit 32 NOOP);
+                ("index_1", P4Bit index_w (Znth 0 (`is)));
+                ("index_2", P4Bit index_w (Znth 1 (`is)));
+                ("index_3", P4Bit index_w (Znth 2 (`is)));
+                ("index_4", P4Bit index_w (Znth 3 (`is)));
+                ("rw_1", P4Bit_ value_w);
+                ("rw_2", P4Bit_ value_w);
+                ("rw_3", P4Bit_ value_w);
+                ("rw_4", P4Bit_ value_w)
+               ]
+        ] ValBaseNull
+        (MEM []
+        (EXT [frame_repr p rows f]))).
+
+Lemma Win_noop_body :
+  func_sound ge Win_fundef nil Win_noop_spec.
+Proof.
+  start_function.
+  unfold frame_repr.
+  normalize_EXT.
+  destruct f as [f ?H]. destruct is as [is ?H].
+  cbn [proj1_sig] in *.
+  destruct_list f.
+  destruct_list is.
+  repeat lazymatch goal with
+  | H : Forall _ _ |- _ => inv H
+  end.
+  step_call verif_Row11.Row_noop_case_body.
+  { entailer. }
+  { auto. }
+  step_call verif_Row12.Row_noop_case_body.
+  { entailer. }
+  { auto. }
+  step_call verif_Row13.Row_noop_case_body.
+  { entailer. }
+  { auto. }
+  step_call verif_Row14.Row_noop_case_body.
+  { entailer. }
+  { auto. }
+  step_call tbl_merge_rows_1_undef_body.
+  { entailer. }
+  Intros _.
+  step_call tbl_merge_rows_2_undef_body.
+  { entailer. }
+  Intros _.
+  step.
+  entailer.
+Qed.
+
+Definition Win_insert_spec : func_spec :=
+  WITH (* p *),
+    PATH p
+    MOD None [p]
+    WITH (f : frame) (is : listn Z num_rows)
+      (_ : Forall (fun i => 0 <= i < num_slots) (`is)),
+      PRE
+        (ARG [ValBaseStruct
+               [("api_call", P4Bit 32 INSERT);
+                ("index_1", P4Bit index_w (Znth 0 (`is)));
+                ("index_2", P4Bit index_w (Znth 1 (`is)));
+                ("index_3", P4Bit index_w (Znth 2 (`is)));
+                ("index_4", P4Bit index_w (Znth 3 (`is)));
+                ("rw_1", P4Bit_ value_w);
+                ("rw_2", P4Bit_ value_w);
+                ("rw_3", P4Bit_ value_w);
+                ("rw_4", P4Bit_ value_w)
+               ]
+             ]
+        (MEM []
+        (EXT [frame_repr p rows f])))
+      POST
+        (ARG_RET [ValBaseStruct
+               [("api_call", P4Bit 32 INSERT);
+                ("index_1", P4Bit index_w (Znth 0 (`is)));
+                ("index_2", P4Bit index_w (Znth 1 (`is)));
+                ("index_3", P4Bit index_w (Znth 2 (`is)));
+                ("index_4", P4Bit index_w (Znth 3 (`is)));
+                ("rw_1", P4Bit_ value_w);
+                ("rw_2", P4Bit_ value_w);
+                ("rw_3", P4Bit_ value_w);
+                ("rw_4", P4Bit_ value_w)
+               ]
+        ] ValBaseNull
+        (MEM []
+        (EXT [frame_repr p rows (frame_insert f is)]))).
+
+Lemma Win_insert_body :
+  func_sound ge Win_fundef nil Win_insert_spec.
+Proof.
+  start_function.
+  unfold frame_repr.
+  normalize_EXT.
+  destruct f as [f ?H]. destruct is as [is ?H].
+  cbn [proj1_sig frame_insert] in *.
+  destruct_list f.
+  destruct_list is.
+  repeat lazymatch goal with
+  | H : Forall _ _ |- _ => inv H
+  end.
+  step_call verif_Row11.Row_insert_case_body.
+  { entailer. }
+  { auto. }
+  step_call verif_Row12.Row_insert_case_body.
+  { entailer. }
+  { auto. }
+  step_call verif_Row13.Row_insert_case_body.
+  { entailer. }
+  { auto. }
+  step_call verif_Row14.Row_insert_case_body.
+  { entailer. }
+  { auto. }
+  step_call tbl_merge_rows_1_undef_body.
+  { entailer.
+    repeat constructor.
+  }
+  Intros _.
+  step_call tbl_merge_rows_2_undef_body.
+  { entailer. }
+  Intros _.
+  step.
+  entailer.
+Qed.
+
+Definition Win_query_spec : func_spec :=
+  WITH (* p *),
+    PATH p
+    MOD None [p]
+    WITH (f : frame) (is : listn Z num_rows)
+      (_ : Forall (fun i => 0 <= i < num_slots) (`is)),
+      PRE
+        (ARG [ValBaseStruct
+               [("api_call", P4Bit 32 QUERY);
+                ("index_1", P4Bit index_w (Znth 0 (`is)));
+                ("index_2", P4Bit index_w (Znth 1 (`is)));
+                ("index_3", P4Bit index_w (Znth 2 (`is)));
+                ("index_4", P4Bit index_w (Znth 3 (`is)));
+                ("rw_1", P4Bit_ value_w);
+                ("rw_2", P4Bit_ value_w);
+                ("rw_3", P4Bit_ value_w);
+                ("rw_4", P4Bit_ value_w)
+               ]
+             ]
+        (MEM []
+        (EXT [frame_repr p rows f])))
+      POST
+        (ARG_RET [ValBaseStruct
+               [("api_call", P4Bit 32 QUERY);
+                ("index_1", P4Bit index_w (Znth 0 (`is)));
+                ("index_2", P4Bit index_w (Znth 1 (`is)));
+                ("index_3", P4Bit index_w (Znth 2 (`is)));
+                ("index_4", P4Bit index_w (Znth 3 (`is)));
+                ("rw_1", P4Bit value_w (frame_query f (`is)));
+                ("rw_2", P4Bit_ value_w);
+                ("rw_3", P4Bit_ value_w);
+                ("rw_4", P4Bit_ value_w)
+               ]
+        ] ValBaseNull
+        (MEM []
+        (EXT [frame_repr p rows f]))).
+
+Lemma Win_query_body :
+  func_sound ge Win_fundef nil Win_query_spec.
+Proof.
+  start_function.
+  unfold frame_repr.
+  normalize_EXT.
+  destruct f as [f ?H]. destruct is as [is ?H].
+  cbn [proj1_sig] in *.
+  destruct_list f.
+  destruct_list is.
+  repeat lazymatch goal with
+  | H : Forall _ _ |- _ => inv H
+  end.
+  step_call verif_Row11.Row_query_case_body.
+  { entailer. }
+  { auto. }
+  step_call verif_Row12.Row_query_case_body.
+  { entailer. }
+  { auto. }
+  step_call verif_Row13.Row_query_case_body.
+  { entailer. }
+  { auto. }
+  step_call verif_Row14.Row_query_case_body.
+  { entailer. }
+  { auto. }
+  step_call tbl_merge_rows_1_body.
+  { entailer. }
+  Intros _.
+  step_call tbl_merge_rows_2_body.
+  { entailer. }
+  Intros _.
+  step.
+  entailer.
+  constructor.
+  repeat first [
+    apply Forall2_nil
+  | apply Forall2_cons; only 1 : (split; only 1 : reflexivity);
+    try apply sval_refine_refl
+  ].
+  2-4 : repeat constructor.
+  apply sval_refine_refl'. repeat f_equal.
+  admit. (* arith *)
+(* Qed. *)
+Admitted.
+
+Definition Win_clear_spec : func_spec :=
+  WITH (* p *),
+    PATH p
+    MOD None [p]
+    WITH (f : frame) (is : listn Z num_rows)
+      (_ : Forall (fun i => 0 <= i < num_slots) (`is)),
+      PRE
+        (ARG [ValBaseStruct
+               [("api_call", P4Bit 32 CLEAR);
+                ("index_1", P4Bit index_w (Znth 0 (`is)));
+                ("index_2", P4Bit index_w (Znth 1 (`is)));
+                ("index_3", P4Bit index_w (Znth 2 (`is)));
+                ("index_4", P4Bit index_w (Znth 3 (`is)));
+                ("rw_1", P4Bit_ value_w);
+                ("rw_2", P4Bit_ value_w);
+                ("rw_3", P4Bit_ value_w);
+                ("rw_4", P4Bit_ value_w)
+               ]
+             ]
+        (MEM []
+        (EXT [frame_repr p rows f])))
+      POST
+        (ARG_RET [ValBaseStruct
+               [("api_call", P4Bit 32 CLEAR);
+                ("index_1", P4Bit index_w (Znth 0 (`is)));
+                ("index_2", P4Bit index_w (Znth 1 (`is)));
+                ("index_3", P4Bit index_w (Znth 2 (`is)));
+                ("index_4", P4Bit index_w (Znth 3 (`is)));
+                ("rw_1", P4Bit_ value_w);
+                ("rw_2", P4Bit_ value_w);
+                ("rw_3", P4Bit_ value_w);
+                ("rw_4", P4Bit_ value_w)
+               ]
+        ] ValBaseNull
+        (MEM []
+        (EXT [frame_repr p rows (frame_clear f is)]))).
+
+Lemma Win_clear_body :
+  func_sound ge Win_fundef nil Win_clear_spec.
+Proof.
+  start_function.
+  unfold frame_repr.
+  normalize_EXT.
+  destruct f as [f ?H]. destruct is as [is ?H].
+  cbn [proj1_sig frame_clear] in *.
+  destruct_list f.
+  destruct_list is.
+  repeat lazymatch goal with
+  | H : Forall _ _ |- _ => inv H
+  end.
+  step_call verif_Row11.Row_clear_case_body.
+  { entailer. }
+  { auto. }
+  step_call verif_Row12.Row_clear_case_body.
+  { entailer. }
+  { auto. }
+  step_call verif_Row13.Row_clear_case_body.
+  { entailer. }
+  { auto. }
+  step_call verif_Row14.Row_clear_case_body.
+  { entailer. }
+  { auto. }
+  step_call tbl_merge_rows_1_undef_body.
+  { entailer.
+    repeat constructor.
+  }
+  Intros _.
+  step_call tbl_merge_rows_2_undef_body.
+  { entailer. }
+  Intros _.
+  step.
+  entailer.
+Qed.
+
+#[export] Hint Extern 5 (func_modifies _ _ _ _ _) => (apply Win_noop_body) : func_specs.
+
+Definition Win_spec : func_spec :=
+  WITH (* p *),
+    PATH p
+    MOD None [p]
+    WITH (op : Z) (f : frame) (is : listn Z num_rows)
+      (_ : In op [NOOP; CLEAR; INSERT; QUERY])
+      (_ : Forall (fun i => 0 <= i < num_slots) (`is)),
+      PRE
+        (ARG [ValBaseStruct
+               [("api_call", P4Bit 32 op);
+                ("index_1", P4Bit index_w (Znth 0 (`is)));
+                ("index_2", P4Bit index_w (Znth 1 (`is)));
+                ("index_3", P4Bit index_w (Znth 2 (`is)));
+                ("index_4", P4Bit index_w (Znth 3 (`is)));
+                ("rw_1", P4Bit_ value_w);
+                ("rw_2", P4Bit_ value_w);
+                ("rw_3", P4Bit_ value_w);
+                ("rw_4", P4Bit_ value_w)
+               ]
+             ]
+        (MEM []
+        (EXT [frame_repr p rows f])))
+      POST
+        (ARG_RET [
+          if op =? NOOP then
+            ValBaseStruct
+              [("api_call", P4Bit 32 NOOP);
+               ("index_1", P4Bit index_w (Znth 0 (`is)));
+               ("index_2", P4Bit index_w (Znth 1 (`is)));
+               ("index_3", P4Bit index_w (Znth 2 (`is)));
+               ("index_4", P4Bit index_w (Znth 3 (`is)));
+               ("rw_1", P4Bit_ value_w);
+               ("rw_2", P4Bit_ value_w);
+               ("rw_3", P4Bit_ value_w);
+               ("rw_4", P4Bit_ value_w)
+              ]
+          else if op =? CLEAR then
+            ValBaseStruct
+              [("api_call", P4Bit 32 CLEAR);
+               ("index_1", P4Bit index_w (Znth 0 (`is)));
+               ("index_2", P4Bit index_w (Znth 1 (`is)));
+               ("index_3", P4Bit index_w (Znth 2 (`is)));
+               ("index_4", P4Bit index_w (Znth 3 (`is)));
+               ("rw_1", P4Bit_ value_w);
+               ("rw_2", P4Bit_ value_w);
+               ("rw_3", P4Bit_ value_w);
+               ("rw_4", P4Bit_ value_w)
+              ]
+          else if op =? INSERT then
+            ValBaseStruct
+              [("api_call", P4Bit 32 INSERT);
+               ("index_1", P4Bit index_w (Znth 0 (`is)));
+               ("index_2", P4Bit index_w (Znth 1 (`is)));
+               ("index_3", P4Bit index_w (Znth 2 (`is)));
+               ("index_4", P4Bit index_w (Znth 3 (`is)));
+               ("rw_1", P4Bit_ value_w);
+               ("rw_2", P4Bit_ value_w);
+               ("rw_3", P4Bit_ value_w);
+               ("rw_4", P4Bit_ value_w)
+              ]
+          else
+            ValBaseStruct
+              [("api_call", P4Bit 32 QUERY);
+               ("index_1", P4Bit index_w (Znth 0 (`is)));
+               ("index_2", P4Bit index_w (Znth 1 (`is)));
+               ("index_3", P4Bit index_w (Znth 2 (`is)));
+               ("index_4", P4Bit index_w (Znth 3 (`is)));
+               ("rw_1", P4Bit value_w (frame_query f (`is)));
+               ("rw_2", P4Bit_ value_w);
+               ("rw_3", P4Bit_ value_w);
+               ("rw_4", P4Bit_ value_w)
+              ]
+        ] ValBaseNull
+        (MEM []
+        (EXT [frame_repr p rows (
+          if op =? NOOP then
+            f
+          else if op =? CLEAR then
+            frame_clear f is
+          else if op =? INSERT then
+            frame_insert f is
+          else
+            f
+        )]))).
+
+Lemma Win_body :
+  func_sound ge Win_fundef nil Win_spec.
+Proof.
+  intros_fs_bind.
+  split; only 2 : solve_modifies.
+  intros_fsh_bind.
+  destruct H.
+  { subst.
+    apply Win_noop_body; auto.
+  }
+  destruct H.
+  { subst.
+    apply Win_clear_body; auto.
+  }
+  destruct H.
+  { subst.
+    apply Win_insert_body; auto.
+  }
+  destruct H.
+  { subst.
+    apply Win_query_body; auto.
+  }
+  destruct H.
+Qed.
