examples/cms/gen_verif_full.sh
@@ -1,0 +1,78 @@
+#!/bin/bash
+
+cd $( dirname -- "$0"; )
+
+cp verif_Row11.v verif_Row12.v
+sed -i.bak 's/\["pipe"; "ingress"; "cm2_ds"; "win_1"; "row_1"\]/\["pipe"; "ingress"; "cm2_ds"; "win_1"; "row_2"\]/' verif_Row12.v
+rm verif_Row12.v.bak
+
+cp verif_Row11.v verif_Row13.v
+sed -i.bak 's/\["pipe"; "ingress"; "cm2_ds"; "win_1"; "row_1"\]/\["pipe"; "ingress"; "cm2_ds"; "win_1"; "row_3"\]/' verif_Row13.v
+rm verif_Row13.v.bak
+
+cp verif_Row11.v verif_Row14.v
+sed -i.bak 's/\["pipe"; "ingress"; "cm2_ds"; "win_1"; "row_1"\]/\["pipe"; "ingress"; "cm2_ds"; "win_1"; "row_4"\]/' verif_Row14.v
+rm verif_Row14.v.bak
+
+cp verif_Row11.v verif_Row21.v
+sed -i.bak 's/\["pipe"; "ingress"; "cm2_ds"; "win_1"; "row_1"\]/\["pipe"; "ingress"; "cm2_ds"; "win_2"; "row_1"\]/' verif_Row21.v
+rm verif_Row21.v.bak
+
+cp verif_Row11.v verif_Row22.v
+sed -i.bak 's/\["pipe"; "ingress"; "cm2_ds"; "win_1"; "row_1"\]/\["pipe"; "ingress"; "cm2_ds"; "win_2"; "row_2"\]/' verif_Row22.v
+rm verif_Row22.v.bak
+
+cp verif_Row11.v verif_Row23.v
+sed -i.bak 's/\["pipe"; "ingress"; "cm2_ds"; "win_1"; "row_1"\]/\["pipe"; "ingress"; "cm2_ds"; "win_2"; "row_3"\]/' verif_Row23.v
+rm verif_Row23.v.bak
+
+cp verif_Row11.v verif_Row24.v
+sed -i.bak 's/\["pipe"; "ingress"; "cm2_ds"; "win_1"; "row_1"\]/\["pipe"; "ingress"; "cm2_ds"; "win_2"; "row_4"\]/' verif_Row24.v
+rm verif_Row24.v.bak
+
+cp verif_Row11.v verif_Row31.v
+sed -i.bak 's/\["pipe"; "ingress"; "cm2_ds"; "win_1"; "row_1"\]/\["pipe"; "ingress"; "cm2_ds"; "win_3"; "row_1"\]/' verif_Row31.v
+rm verif_Row31.v.bak
+
+cp verif_Row11.v verif_Row32.v
+sed -i.bak 's/\["pipe"; "ingress"; "cm2_ds"; "win_1"; "row_1"\]/\["pipe"; "ingress"; "cm2_ds"; "win_3"; "row_2"\]/' verif_Row32.v
+rm verif_Row32.v.bak
+
+cp verif_Row11.v verif_Row33.v
+sed -i.bak 's/\["pipe"; "ingress"; "cm2_ds"; "win_1"; "row_1"\]/\["pipe"; "ingress"; "cm2_ds"; "win_3"; "row_3"\]/' verif_Row33.v
+rm verif_Row33.v.bak
+
+cp verif_Row11.v verif_Row34.v
+sed -i.bak 's/\["pipe"; "ingress"; "cm2_ds"; "win_1"; "row_1"\]/\["pipe"; "ingress"; "cm2_ds"; "win_3"; "row_4"\]/' verif_Row34.v
+rm verif_Row34.v.bak
+
+cp verif_Row11.v verif_Row41.v
+sed -i.bak 's/\["pipe"; "ingress"; "cm2_ds"; "win_1"; "row_1"\]/\["pipe"; "ingress"; "cm2_ds"; "win_4"; "row_1"\]/' verif_Row41.v
+rm verif_Row41.v.bak
+
+cp verif_Row11.v verif_Row42.v
+sed -i.bak 's/\["pipe"; "ingress"; "cm2_ds"; "win_1"; "row_1"\]/\["pipe"; "ingress"; "cm2_ds"; "win_4"; "row_2"\]/' verif_Row42.v
+rm verif_Row42.v.bak
+
+cp verif_Row11.v verif_Row43.v
+sed -i.bak 's/\["pipe"; "ingress"; "cm2_ds"; "win_1"; "row_1"\]/\["pipe"; "ingress"; "cm2_ds"; "win_4"; "row_3"\]/' verif_Row43.v
+rm verif_Row43.v.bak
+
+cp verif_Row11.v verif_Row44.v
+sed -i.bak 's/\["pipe"; "ingress"; "cm2_ds"; "win_1"; "row_1"\]/\["pipe"; "ingress"; "cm2_ds"; "win_4"; "row_4"\]/' verif_Row44.v
+rm verif_Row44.v.bak
+
+cp verif_Win1.v verif_Win2.v
+sed -i.bak 's/\["pipe"; "ingress"; "cm2_ds"; "win_1"\]/\["pipe"; "ingress"; "cm2_ds"; "win_2"\]/' verif_Win2.v
+sed -i.bak 's/verif_Row1/verif_Row2/' verif_Win2.v
+rm verif_Win2.v.bak
+
+cp verif_Win1.v verif_Win3.v
+sed -i.bak 's/\["pipe"; "ingress"; "cm2_ds"; "win_1"\]/\["pipe"; "ingress"; "cm2_ds"; "win_3"\]/' verif_Win3.v
+sed -i.bak 's/verif_Row1/verif_Row3/' verif_Win3.v
+rm verif_Win3.v.bak
+
+cp verif_Win1.v verif_Win4.v
+sed -i.bak 's/\["pipe"; "ingress"; "cm2_ds"; "win_1"\]/\["pipe"; "ingress"; "cm2_ds"; "win_4"\]/' verif_Win4.v
+sed -i.bak 's/verif_Row1/verif_Row4/' verif_Win4.v
+rm verif_Win4.v.bak
